LeanSubst/Basic.lean
@@ -1,4 +1,4 @@
-
+import Lilac
 -- TODO:
 -- Generalizing to vector substitutions is a matter of the following change:
 -- `SubstMap S T` becomes `SubstMap n S (T n)` for `T : Nat -> Type`
@@ -12,25 +12,16 @@ namespace LeanSubst
   universe u
   variable {S T : Type}
 
-  @[simp]
-  def Sequence.cons {T : Type u} (x : T) (xs : Nat -> T) : Nat -> T
-  | 0 => x
-  | n + 1 => xs n
+  def Ren := Sequ Nat
 
-  infixr:55 "::" => Sequence.cons
-
-  def Endo (T : Type) := T -> T
-
-  abbrev Ren := Nat -> Nat
-
-  def Ren.lift : Endo Ren
+  def Ren.lift : Ren -> Ren
   | _, 0 => 0
   | r, n + 1 => r n + 1
 
   class RenMap (T : Type) where
-    rmap : Endo Ren -> Ren -> T -> T
+    rmap : Ren -> T -> T
 
-  def Ren.apply [RenMap T] (r : Ren) : T -> T := RenMap.rmap Ren.lift r
+  export RenMap (rmap)
 
   inductive Subst.Action (T : Type) where
   | re : Nat -> Subst.Action T
@@ -39,7 +30,7 @@ namespace LeanSubst
 
   export Subst.Action (re su)
 
-  abbrev Subst (T : Type) := Nat -> Subst.Action T
+  def Subst (T : Type) := Sequ $ Subst.Action T
 
   @[coe]
   def Ren.to : Ren -> Subst T
@@ -49,29 +40,30 @@ namespace LeanSubst
     coe := Ren.to
 
   class SubstMap (S T : Type) where
-    smap : Endo (Subst T) -> Subst T -> S -> S
+    smap : Subst T -> S -> S
 
-  def Subst.lift [RenMap T] : Endo (Subst T)
+  export SubstMap (smap)
+
+  def Subst.lift [RenMap T] : Subst T -> Subst T
   | _, 0 => re 0
   | σ, n + 1 =>
     match σ n with
-    | su t => su (Ren.apply (· + 1) t)
+    | su t => su (rmap (· + 1) t)
     | re k => re (k + 1)
 
-  def Subst.apply [RenMap T] [SubstMap S T] (σ : Subst T) : S -> S := SubstMap.smap Subst.lift σ
-
-  abbrev Subst.apply1 [RenMap S] [SubstMap S S] := Subst.apply (S := S) (T := S)
+  @[simp]
+  abbrev smap1 [SubstMap S S] := smap (S := S) (T := S)
 
   def Subst.compose [RenMap T] [SubstMap T T] : Subst T -> Subst T -> Subst T
   | σ, τ, n =>
     match σ n with
-    | su t => su (apply τ t)
+    | su t => su (smap τ t)
     | re k => τ k
 
   def Subst.hcompose [RenMap T] [SubstMap S T] : Subst S -> Subst T -> Subst S
   | σ, τ, n =>
     match σ n with
-    | su t => su (apply τ t)
+    | su t => su (smap τ t)
     | re k => re k
 
   def Subst.id : Subst T := λ n => re n
@@ -112,23 +104,38 @@ namespace LeanSubst
     unfold Subst.id; rfl
 
   @[simp]
+  theorem Ren.to_lift [RenMap T] {r : Ren} : r.lift.to = (@Ren.to T r).lift := by
+    funext; case _ x =>
+    cases x
+    case zero =>
+      unfold Ren.to; unfold Ren.lift; simp
+      unfold Subst.lift; simp
+    case _ n =>
+      generalize lhsdef : ((@Ren.to T r.lift)) (n + 1) = lhs
+      generalize rhsdef : ((@Ren.to T r).lift) (n + 1) = rhs
+      unfold Ren.to at lhsdef; simp at *
+      unfold Ren.lift at lhsdef; simp at *
+      unfold Subst.lift at rhsdef; simp at *
+      subst lhsdef; subst rhsdef; rfl
+
+  @[simp]
   theorem Ren.to_compose {r1 r2 : Ren} [RenMap T] [SubstMap T T]
     : Ren.to (T := T) (r2 ∘ r1) = Subst.compose r1 r2
   := by
     funext; case _ x =>
     cases x <;> simp [Ren.to, Subst.compose]
 
-  macro:max t:term noWs "[" σ:term "]" : term => `(Subst.apply1 $σ $t)
-  macro:max t:term noWs "[" σ:term ":" T:term "]" : term => `(Subst.apply (T := $T) $σ $t)
+  macro:max t:term noWs "[" σ:term "]" : term => `(smap1 $σ $t)
+  macro:max t:term noWs "[" σ:term ":" T:term "]" : term => `(smap (T := $T) $σ $t)
   infixr:85 " ∘ " => Subst.compose
   infixr:85 " ◾ " => Subst.hcompose
 
-  @[app_unexpander Subst.apply1]
+  @[app_unexpander smap1]
   def unexpandSubstApply1 : Lean.PrettyPrinter.Unexpander
   | `($_ $σ $t) => `($t[$σ])
   | _ => throw ()
 
-  @[app_unexpander Subst.apply]
+  @[app_unexpander smap]
   def unexpandSubstApply : Lean.PrettyPrinter.Unexpander
   | `($_ $σ $t) => `($t[$σ : _])
   | `($_ (T := $T) $σ $t) => `($t[$σ : $T])
