Examples/IntrinsicStlc.lean
@@ -1,0 +1,55 @@
+
+inductive Ty where
+| base : Ty
+| arrow : Ty -> Ty -> Ty
+
+notation "★" => Ty.base
+infixr:78 " -:> " => Ty.arrow
+
+inductive Var : List Ty -> Ty -> Type where
+| here {Γ A} : Var (A::Γ) A
+| there {Γ A B} : Var Γ B -> Var (A::Γ) B
+
+inductive Term : List Ty -> Ty -> Type where
+| var {Γ T} :
+  Var Γ T ->
+  Term Γ T
+| lam {Γ A B} :
+  Term (A::Γ) B ->
+  Term Γ (A -:> B)
+| app {Γ A B} :
+  Term Γ (A -:> B) ->
+  Term Γ A ->
+  Term Γ B
+
+def Ren (Γ Δ : List Ty) := ∀ {T}, Var Γ T -> Var Δ T
+
+def Ren.lift {Γ Δ : List Ty} (r : Ren Γ Δ) {T : Ty} : Ren (T::Γ) (T::Δ)
+| _, .here => .here
+| _, .there x => .there (r x)
+
+def Term.rmap {Γ Δ : List Ty} (r : Ren Γ Δ) {T : Ty} : Term Γ T -> Term Δ T
+| var v => var (r v)
+| lam t => lam (rmap (Ren.lift r) t)
+| app f a => app (rmap r f) (rmap r a)
+
+inductive Action (Γ : List Ty) (T : Ty) : Type where
+| re : Var Γ T -> Action Γ T
+| su : Term Γ T -> Action Γ T
+
+def Subst (Γ Δ : List Ty) := ∀ {T}, Var Γ T -> Action Δ T
+
+def Subst.lift {Γ Δ : List Ty} (σ : Subst Γ Δ) {T : Ty} : Subst (T::Γ) (T::Δ)
+| _, .here => .re .here
+| _, .there x =>
+  match σ x with
+  | .su t => .su (Term.rmap .there t)
+  | .re k => .re (.there k)
+
+def Term.smap {Γ Δ : List Ty} (σ : Subst Γ Δ) {T : Ty} : Term Γ T -> Term Δ T
+| var v =>
+  match σ v with
+  | .su t => t
+  | .re k => var k
+| lam t => lam (smap (Subst.lift σ) t)
+| app f a => app (smap σ f) (smap σ a)
