LeanSubst.lean
@@ -1,6 +1,7 @@
 
 import LeanSubst.Basic
 import LeanSubst.Laws
+import LeanSubst.Option
 import LeanSubst.List
 import LeanSubst.Reduction
 import LeanSubst.Normal
