LeanSubst/Generic.lean
@@ -1,0 +1,44 @@
+
+-- universe u u1 u2 u3 u4
+
+-- class SyntaxStructure (Ctx : Type u1) (S : Ctx -> Type u2) where
+--   Var : Ctx -> Type u2
+--   Ren : (Ctx -> Type u2) -> Ctx -> Ctx -> Sort u3
+--   Lift : (Ctx -> Ctx -> Sort u3) -> Ctx -> Ctx -> Sort u3
+--   rlift {Γ Δ : Ctx} : Ren Var Γ Δ -> Lift (Ren Var) Γ Δ
+--   rmap {Γ Δ : Ctx} (r : Ren Var Γ Δ) : Ren S Γ Δ
+
+
+
+-- inductive Ty where
+-- | base : Ty
+-- | arrow : Ty -> Ty -> Ty
+
+-- notation "★" => Ty.base
+-- infixr:78 " -:> " => Ty.arrow
+
+-- inductive Var : List Ty -> Ty -> Type where
+-- | here {Γ A} : Var (A::Γ) A
+-- | there {Γ A B} : Var Γ B -> Var (A::Γ) B
+
+-- inductive Term : List Ty -> Ty -> Type where
+-- | var {Γ T} :
+--   Var Γ T ->
+--   Term Γ T
+-- | lam {Γ A B} :
+--   Term (A::Γ) B ->
+--   Term Γ (A -:> B)
+-- | app {Γ A B} :
+--   Term Γ (A -:> B) ->
+--   Term Γ A ->
+--   Term Γ B
+
+-- instance : SyntaxStructure (List Ty) ((A : Ty) -> Term · A) where
+--   Var Γ := (A : Ty) -> Var Γ A
+--   Ren F Γ Δ := {A : Ty} -> F Γ -> F Δ
+--   Lift
+
+-- open SyntaxStructure
+
+-- class RenMap [SyntaxStructure] (S : Ctx Idx -> Idx -> Type u3) where
+--   rmap {Γ Δ : Ctx Idx} (r : Ren Γ Δ) {T : Idx} : S Γ T -> S Δ T
