LeanSubst/Option.lean
@@ -1,0 +1,24 @@
+import LeanSubst.Basic
+
+namespace LeanSubst
+
+variable {S T : Type}
+
+def Option.smap [SubstMap S T] (σ : Subst T) : Option S -> Option S
+| none => none
+| some t => some t[σ:_]
+
+instance [SubstMap S T] : SubstMap (Option S) T where
+  smap := Option.smap
+
+@[simp]
+theorem Option.smap_none [SubstMap S T] {σ : Subst T}
+  : (@Option.none S)[σ:_] = none
+:= by
+  simp [SubstMap.smap, Option.smap]
+
+@[simp]
+theorem Option.smap_some [SubstMap S T] {x : S} {σ : Subst T}
+  : (some x)[σ:_] = some x[σ:_]
+:= by
+  simp [SubstMap.smap, Option.smap]
